AVM/Program/Parameters.lean
@@ -1,0 +1,84 @@
+import AVM.Object
+
+namespace AVM
+
+inductive Program.Parameters where
+  | empty
+  | fetch (param : TypedObjectId) (rest : Object param.classLabel → Program.Parameters)
+  | genId (rest : ObjectId → Program.Parameters)
+deriving Inhabited
+
+def Program.Parameters.Product (params : Program.Parameters) : Type u :=
+  match params with
+  | .empty => PUnit
+  | .fetch param rest =>
+    Σ (obj : Object param.classLabel), Program.Parameters.Product (rest obj)
+  | .genId rest =>
+    Σ (objId : ObjectId), Program.Parameters.Product (rest objId)
+
+instance {params : Program.Parameters} : TypeRep params.Product where
+  rep := Rep.atomic "Program.Parameters.Product" -- TODO: this should depend on params
+
+namespace Program.Parameters
+
+def Product.beq {params : Program.Parameters} (a b : params.Product) :=
+    match params with
+    | .empty => true
+    | .fetch _ _ =>
+      let ⟨objA, valsA⟩ := a
+      let ⟨objB, valsB⟩ := b
+      check objA == objB
+      let try valsB' := tryCast valsB
+      beq valsA valsB'
+    | .genId _ =>
+      let ⟨objIdA, valsA⟩ := a
+      let ⟨objIdB, valsB⟩ := b
+      check objIdA == objIdB
+      let try valsB' := tryCast valsB
+      beq valsA valsB'
+
+instance {params : Program.Parameters} : BEq params.Product where
+  beq := Program.Parameters.Product.beq
+
+def append (params1 : Program.Parameters) (params2 : params1.Product → Program.Parameters) : Program.Parameters :=
+  match params1 with
+  | .empty =>
+    params2 PUnit.unit
+  | .fetch p1 ps1 =>
+    .fetch p1
+      (fun obj => (ps1 obj).append (fun vals => params2 ⟨obj, vals⟩))
+  | .genId ps1 =>
+    .genId (fun objId => (ps1 objId).append (fun vals => params2 ⟨objId, vals⟩))
+
+def concat (params : List Program.Parameters) : Program.Parameters :=
+  match params with
+  | [] => .empty
+  | ps :: rest =>
+    ps.append (fun _ => concat rest)
+
+def splitProduct
+  {params1 : Program.Parameters}
+  {params2 : params1.Product → Program.Parameters}
+  (vals : params1.append params2 |>.Product)
+  : Σ (vals : params1.Product), (params2 vals).Product :=
+  match params1 with
+  | .empty => ⟨PUnit.unit, vals⟩
+  | .fetch _ _ =>
+    let ⟨obj, vals'⟩ := vals
+    let ⟨vals1, vals2⟩ := splitProduct vals'
+    ⟨⟨obj, vals1⟩, vals2⟩
+  | .genId _ =>
+    let ⟨objId, vals'⟩ := vals
+    let ⟨vals1, vals2⟩ := splitProduct vals'
+    ⟨⟨objId, vals1⟩, vals2⟩
+
+def splitProducts
+  {params : List Program.Parameters}
+  (vals : Program.Parameters.concat params |>.Product)
+  : HList (params.map Program.Parameters.Product) :=
+  match params with
+  | [] => HList.nil
+  | _ :: ps =>
+    let ⟨vals1, vals'⟩ := splitProduct vals
+    let rest : HList (ps.map Program.Parameters.Product) := splitProducts vals'
+    HList.cons vals1 rest
