Applib/Surface/Program/Syntax.lean
@@ -8,34 +8,22 @@ declare_syntax_cat program
 
 syntax withPosition("create " ident ident term) optSemicolon(program) : program
 syntax withPosition(ident " := " " create " ident ident term) optSemicolon(program) : program
-syntax withPosition("destroy " ident ident term) optSemicolon(program) : program
-syntax withPosition("call " ident ident term) optSemicolon(program) : program
+syntax withPosition("destroy " ident term) optSemicolon(program) : program
+syntax withPosition("call " ident term) optSemicolon(program) : program
 syntax withPosition(ident " := " " fetch " term) optSemicolon(program) : program
 syntax "return " term : program
-syntax "Ξ " ident* " . " program:40 : term
 syntax "⟪" program "⟫" : term
 
-def mkProducts {m} [Monad m] [MonadQuotation m] (ss : TSyntaxArray `ident) : m (TSyntax `term) := do
-  let unit : TSyntax `term ← `(_)
-  ss.foldrM (fun s acc => `(⟨$s, $acc⟩)) unit
-
 macro_rules
-  | `(⟪$p:program⟫) => `(Ξ . $p)
-  | `(Ξ $ss:ident* . create $c:ident $m:ident $e:term ; $p:program) => do
-    let ps ← mkProducts ss
-    `(Program.create $c $m (fun $ps => $e) (Ξ $ss* __ . $p))
-  | `(Ξ $ss:ident* . $x:ident := create $c:ident $m:ident $e:term ; $p:program) => do
-    let ps ← mkProducts ss
-    `(Program.create $c $m (fun $ps => $e) (Ξ $ss* $x . $p))
-  | `(Ξ $ss:ident* . destroy $c:ident $m:ident $e:term $args:term ; $p:program) => do
-    let ps ← mkProducts ss
-    `(Program.destroy $c $m (fun $ps => $e) (fun $ps => $args) (Ξ $ss* . $p))
-  | `(Ξ $ss:ident* . call $c:ident $m:ident $e:term $args:term ; $p:program) => do
-    let ps ← mkProducts ss
-    `(Program.call $c $m (fun $ps => $e) (fun $ps => $args) (Ξ $ss* . $p))
-  | `(Ξ $ss:ident* . $x:ident := fetch $e:term ; $p:program) => do
-    let ps ← mkProducts ss
-    `(Program.fetch (fun $ps => $e) (Ξ $ss* $x . $p))
-  | `(Ξ $ss:ident* . return $e:term) => do
-    let ps ← mkProducts ss
-    `(Program.return (fun $ps => $e))
+  | `(⟪create $c:ident $m:ident $e:term ; $p:program⟫) => do
+    `(Program.create' $c $m $e (fun _ => ⟪$p⟫))
+  | `(⟪$x:ident := create $c:ident $m:ident $e:term ; $p:program⟫) => do
+    `(Program.create' $c $m $e (fun $x => ⟪$p⟫))
+  | `(⟪destroy $m:ident $e:term $args:term ; $p:program⟫) => do
+    `(Program.destroy' $e $m $args ⟪$p⟫)
+  | `(⟪call $m:ident $e:term $args:term ; $p:program⟫) => do
+    `(Program.call' $e $m $args ⟪$p⟫)
+  | `(⟪$x:ident := fetch $e:term ; $p:program⟫) => do
+    `(Program.fetch' $e (fun $x => ⟪$p⟫))
+  | `(⟪return $e:term⟫) => do
+    `(Program.return $e)
