Tests/Applib/Surface/Program/Syntax.lean
@@ -9,24 +9,24 @@ open Applib
 example (rx ry : Reference Counter) : Program Eco.lab Counter := ⟪
   x := fetch rx
   y := fetch ry
-  call Counter Counter.Methods.Incr rx (x.count * 2 + y.count)
-  call Counter Counter.Methods.Incr ry (y.count * 2 + x.count)
+  call Counter.Methods.Incr rx (x.count * 2 + y.count)
+  call Counter.Methods.Incr ry (y.count * 2 + x.count)
   return {x with count := x.count + y.count}
 ⟫
 
 example (rx ry : Reference Counter) : Program Eco.lab Unit := ⟪
   x := fetch rx
   y := fetch ry
-  call Counter Counter.Methods.Incr rx (x.count * 2 + y.count)
-  call Counter Counter.Methods.Incr ry (y.count * 2 + x.count)
+  call Counter.Methods.Incr rx (x.count * 2 + y.count)
+  call Counter.Methods.Incr ry (y.count * 2 + x.count)
   return ()
 ⟫
 
 example : Program Eco.lab (Reference TwoCounter) := ⟪
   rx := create Counter Counter.Constructors.Zero ()
   ry := create Counter Counter.Constructors.Zero ()
-  call Counter Counter.Methods.Incr rx (2 : Nat)
-  call Counter Counter.Methods.Incr ry (7 : Nat)
+  call Counter.Methods.Incr rx (2 : Nat)
+  call Counter.Methods.Incr ry (7 : Nat)
   tc := create TwoCounter TwoCounter.Constructors.Zero (rx, ry)
   return tc
 ⟫
@@ -34,8 +34,8 @@ example : Program Eco.lab (Reference TwoCounter) := ⟪
 example (self : TwoCounter) (n : Nat) : Program Eco.lab TwoCounter := ⟪
   c1 := fetch self.c1
   c2 := fetch self.c2
-  call Counter Counter.Methods.Incr self.c1 (c2.count * n + c1.count)
-  call Counter Counter.Methods.Incr self.c2 (c1.count * n + c2.count)
+  call Counter.Methods.Incr self.c1 (c2.count * n + c1.count)
+  call Counter.Methods.Incr self.c2 (c1.count * n + c2.count)
   return self
 ⟫
 
@@ -47,16 +47,16 @@ open Applib
 
 example (r : Reference OwnedCounter) (newOwner : PublicKey) : Program label (Reference OwnedCounter) := ⟪
   c := fetch r
-  call OwnedCounter OwnedCounter.Methods.Transfer r newOwner
+  call OwnedCounter.Methods.Transfer r newOwner
   r' := create OwnedCounter OwnedCounter.Constructors.Zero ()
-  call OwnedCounter OwnedCounter.Methods.Incr r' (c.count + 1)
-  destroy OwnedCounter OwnedCounter.Destructors.Ten r ()
+  call OwnedCounter.Methods.Incr r' (c.count + 1)
+  destroy OwnedCounter.Destructors.Ten r ()
   return r'
 ⟫
 
 example (n : Nat) : Program label (Reference OwnedCounter) := ⟪
   r := create OwnedCounter OwnedCounter.Constructors.Zero ()
-  call OwnedCounter OwnedCounter.Methods.Incr r n
+  call OwnedCounter.Methods.Incr r n
   create OwnedCounter OwnedCounter.Constructors.Zero ()
   create OwnedCounter OwnedCounter.Constructors.Zero ()
   return r
